Got examples compiling and running!

Examples.thy
@@ -10,31 +10,33 @@ definition pred_expr :: expr where
 
 definition greater_than_helper :: expr where
   "greater_than_helper = 
-      IF is_zero_expr \<cdot> \<pi>\<^sub>1 THEN \<iota>\<^sub>l \<cdot> \<kappa> FalseV 
-      ELSE IF is_zero_expr \<cdot> \<pi>\<^sub>2 THEN \<iota>\<^sub>l \<cdot> \<kappa> TrueV 
-      ELSE \<iota>\<^sub>r \<cdot> pred_expr \<parallel> pred_expr 
+      IF (Var ''is_zero'') \<cdot> \<pi>\<^sub>1 THEN \<iota>\<^sub>l \<cdot> \<kappa> FalseV 
+      ELSE IF (Var ''is_zero'') \<cdot> \<pi>\<^sub>2 THEN \<iota>\<^sub>l \<cdot> \<kappa> TrueV 
+      ELSE \<iota>\<^sub>r \<cdot> (Var ''pred'') \<parallel> (Var ''pred'')
       FI FI"
 
 definition greater_than_expr :: expr where
-  "greater_than_expr = \<lparr> \<Xi> \<rparr>\<^bsub>K Bool \<Oplus> Id\<^esub> \<cdot> \<lbrakk> greater_than_helper \<rbrakk>\<^bsub>K Bool \<Oplus> Id\<^esub>"
+  "greater_than_expr = \<lparr> \<Xi> \<rparr>\<^bsub>K Bool \<Oplus> Id\<^esub> \<cdot> \<lbrakk> Var ''greater_than_helper'' \<rbrakk>\<^bsub>K Bool \<Oplus> Id\<^esub>"
 
 definition length_expr :: "type \<Rightarrow> expr" ("length\<^bsub>_\<^esub>") where
   "length\<^bsub>t\<^esub> = \<lparr> \<kappa> ZeroV \<nabla> (succ \<cdot> \<pi>\<^sub>2) \<rparr>\<^bsub>ListF t\<^esub>"
 
-lemma "algorithmic_typecheck is_zero_expr = Some (Nat \<hookrightarrow> Bool)"
+lemma "algorithmic_typecheck\<^sub>e Map.empty is_zero_expr = Some (Nat, Bool)"
   by (simp add: is_zero_expr_def Let_def)
 
-lemma [simp]: "algorithmic_typecheck pred_expr = Some (Nat \<hookrightarrow> Nat)"
+lemma [simp]: "algorithmic_typecheck\<^sub>e Map.empty pred_expr = Some (Nat, Nat)"
   by (simp add: pred_expr_def Let_def)
 
-lemma [simp]: "algorithmic_typecheck greater_than_helper = Some (Nat \<otimes> Nat \<hookrightarrow> Bool \<oplus> Nat \<otimes> Nat)"
-  by (simp add: greater_than_helper_def pred_expr_def is_zero_expr_def Let_def)
+lemma [simp]: "algorithmic_typecheck\<^sub>e [''is_zero'' \<mapsto> (Nat, Bool), ''pred'' \<mapsto> (Nat, Nat)] 
+    greater_than_helper = Some (Nat \<otimes> Nat, Bool \<oplus> Nat \<otimes> Nat)"
+  by (simp add: greater_than_helper_def Let_def)
 
-lemma "algorithmic_typecheck greater_than_expr = Some (Nat \<otimes> Nat \<hookrightarrow> Bool)"
-  by (simp add: greater_than_expr_def greater_than_helper_def pred_expr_def is_zero_expr_def Let_def)
+lemma "algorithmic_typecheck\<^sub>e [''greater_than_helper'' \<mapsto> (Nat \<otimes> Nat, Bool \<oplus> Nat \<otimes> Nat)] 
+    greater_than_expr = Some (Nat \<otimes> Nat, Bool)"
+  by (simp add: greater_than_expr_def Let_def)
 
-lemma "algorithmic_typecheck length\<^bsub>t\<^esub> = Some (List t \<hookrightarrow> Nat)"
-  by (simp add: length_expr_def )
+lemma "algorithmic_typecheck\<^sub>e Map.empty length\<^bsub>t\<^esub> = Some (List t, Nat)"
+  by (simp add: length_expr_def Let_def)
 
 primrec nat_to_val :: "nat \<Rightarrow> val" where
   "nat_to_val 0 = ZeroV"
@@ -47,32 +49,38 @@ primrec list_to_val :: "type \<Rightarrow> val list \<Rightarrow> val" where
 abbreviation long_run :: nat where
   "long_run \<equiv> Suc (Suc (Suc (Suc (Suc (Suc (Suc (Suc (Suc (Suc (Suc (Suc 0)))))))))))"
 
-lemma "partial_evaluation \<Lambda> long_run is_zero_expr ZeroV = Some TrueV"
+lemma "partial_eval_prog long_run (Prog [] is_zero_expr ZeroV) = Some TrueV"
   by (simp add: is_zero_expr_def)
 
-lemma "partial_evaluation \<Lambda> long_run is_zero_expr (SuccV ZeroV) = Some FalseV"
+lemma "partial_eval_prog long_run (Prog [] is_zero_expr (SuccV ZeroV)) = Some FalseV"
   by (simp add: is_zero_expr_def)
 
-lemma "partial_evaluation \<Lambda> long_run is_zero_expr (SuccV (SuccV ZeroV)) = Some FalseV"
+lemma "partial_eval_prog long_run (Prog [] is_zero_expr (SuccV (SuccV ZeroV))) = Some FalseV"
   by (simp add: is_zero_expr_def)
 
-lemma "partial_evaluation \<Lambda> long_run pred_expr ZeroV = Some ZeroV"
+lemma "partial_eval_prog long_run (Prog [] pred_expr ZeroV) = Some ZeroV"
   by (simp add: pred_expr_def)
 
-lemma "partial_evaluation \<Lambda> long_run pred_expr (SuccV ZeroV) = Some ZeroV"
+lemma "partial_eval_prog long_run (Prog [] pred_expr (SuccV ZeroV)) = Some ZeroV"
   by (simp add: pred_expr_def)
 
-lemma "partial_evaluation \<Lambda> long_run pred_expr (SuccV (SuccV ZeroV)) = Some (SuccV ZeroV)"
+lemma "partial_eval_prog long_run (Prog [] pred_expr (SuccV (SuccV ZeroV))) = Some (SuccV ZeroV)"
   by (simp add: pred_expr_def)
 
-lemma "partial_evaluation \<Lambda> long_run length\<^bsub>t\<^esub> (list_to_val t [a, b, c]) = 
+lemma "partial_eval_prog long_run (Prog [] length\<^bsub>t\<^esub> (list_to_val t [a, b, c])) = 
     Some (nat_to_val (Suc (Suc (Suc 0))))"
   by (simp add: length_expr_def)
 
-lemma "partial_evaluation \<Lambda> long_run greater_than_expr (PairV (SuccV (SuccV ZeroV)) (SuccV ZeroV)) = Some TrueV"
+abbreviation example_env :: "decl list" where
+  "example_env \<equiv> [
+    ExprDecl ''pred'' pred_expr,
+    ExprDecl ''is_zero'' is_zero_expr,
+    ExprDecl ''greater_than_helper'' greater_than_helper]"
+
+lemma "partial_eval_prog long_run (Prog example_env greater_than_expr (PairV (SuccV (SuccV ZeroV)) (SuccV ZeroV))) = Some TrueV"
   by (simp add: greater_than_expr_def greater_than_helper_def is_zero_expr_def pred_expr_def)
 
-lemma "partial_evaluation \<Lambda> long_run greater_than_expr (PairV (SuccV ZeroV) (SuccV (SuccV ZeroV))) = Some FalseV"
+lemma "partial_eval_prog long_run (Prog example_env greater_than_expr (PairV (SuccV ZeroV) (SuccV (SuccV ZeroV)))) = Some FalseV"
   by (simp add: greater_than_expr_def greater_than_helper_def is_zero_expr_def pred_expr_def)
 
 end
